implemented -fno-postpass normally

mppa_k1c/Asmgen.v
@@ -19,13 +19,16 @@ Require Import Integers.
 Require Import Mach Asm Asmblock Asmblockgen Machblockgen.
 Require Import PostpassScheduling.
 Require Import Errors.
+Require Import Compopts.
 
 Local Open Scope error_monad_scope.
 
 Definition transf_program (p: Mach.program) : res Asm.program :=
   let mbp := Machblockgen.transf_program p in
   do abp <- Asmblockgen.transf_program mbp;
-  do abp' <- PostpassScheduling.transf_program abp;
+    do abp' <- if Compopts.optim_postpass tt
+               then PostpassScheduling.transf_program abp
+               else OK abp;
   OK (Asm.transf_program abp').
 
 Definition transf_function (f: Mach.function) : res Asm.function :=
